src/program_proof/memkv/memkv_shard_proof.v
@@ -2,7 +2,7 @@ From Perennial.program_proof Require Import proof_prelude.
 From Goose.github_com.mit_pdos.gokv Require Import memkv.
 From Perennial.goose_lang Require Import ffi.grove_ffi.
 From Perennial.program_proof.lockservice Require Import rpc.
-From Perennial.program_proof.memkv Require Export memkv_marshal_get_proof common_proof.
+From Perennial.program_proof.memkv Require Export memkv_marshal_get_proof memkv_marshal_install_shard_proof common_proof.
 
 Section memkv_shard_proof.
 
@@ -14,6 +14,7 @@ Global Instance kvptst_tmlss γkv k v : Timeless (kvptsto γkv k v).
 Admitted.
 
 Definition uKV_GET := 2.
+Definition uKV_INS_SHARD := 3.
 
 Record memkv_shard_names := {
  rpc_gn : rpc_names ;
@@ -86,6 +87,16 @@ Definition is_shard_server host γ : iProp Σ :=
                                               ⌜has_encoding_GetRequest reqData req⌝ ∗
                                               (RPCRequestStale γ.(rpc_gn) {| Req_CID:=req.(GR_CID); Req_Seq:=req.(GR_Seq) |} ∨
                                               RPCReplyReceipt γ.(rpc_gn) {| Req_CID:=req.(GR_CID); Req_Seq:=req.(GR_Seq) |} rep)
+             ) (* post *) ∗
+
+  "#HinstallSpec" ∷ handler_is (rpc_request_names) host uKV_INS_SHARD
+             (λ x reqData, ∃ args, ⌜has_encoding_InstallShardRequest reqData args⌝ ∗
+                                  ⌜int.nat args.(IR_Sid) < uNSHARD⌝ ∗
+                                  is_RPCRequest γ.(rpc_gn) x (own_shard γ.(kv_gn) args.(IR_Sid) args.(IR_Kvs))
+                                                            (λ _, True)
+                                                            {| Req_CID:=args.(IR_CID); Req_Seq:=args.(IR_Seq) |}
+             ) (* pre *)
+             (λ x reqData repData, True
              ) (* post *)
 .
 
@@ -502,6 +513,7 @@ Proof.
           }
         }
         iSplitL ""; first done.
+        iSplitL ""; first done.
         iApply "HownShards".
         iRight.
         iExists _, _, _.
@@ -602,117 +614,6 @@ Proof.
     }
   }
 Admitted. (* TODO: evars: into_val.IntoVal GetReplyC *)
-
-Lemma wp_MemKVShardServer__Start (s:loc) host γ :
-is_shard_server host γ -∗
-is_MemKVShardServer s γ -∗
-  {{{
-       True
-  }}}
-    MemKVShardServer__Start #s
-  {{{
-       RET #(); True
-  }}}.
-Proof.
-  iIntros "#His_shard #His_memkv !#" (Φ) "_ HΦ".
-  wp_rec.
-  change (Alloc (InjLV (λ: <>, (λ: <>, #())%V))) with
-      (NewMap grove_common.RawRpcFunc).
-  wp_apply map.wp_NewMap.
-  iIntros (handlers_ptr) "Hmap".
-  wp_pures.
-
-  wp_apply (map.wp_MapInsert with "Hmap").
-  iIntros "Hmap".
-  wp_pures.
-
-  wp_apply (map.wp_MapInsert with "Hmap").
-  iIntros "Hmap".
-  wp_pures.
-
-  wp_apply (map.wp_MapInsert with "Hmap").
-  iIntros "Hmap".
-  wp_pures.
-
-  wp_apply (map.wp_MapInsert with "Hmap").
-  iIntros "Hmap".
-  wp_pures.
-
-  wp_apply (map.wp_MapInsert with "Hmap").
-  iIntros "Hmap".
-  wp_pures.
-
-  wp_apply (grove_ffi.wp_StartRPCServer with "[$Hmap]").
-  {
-    iApply (big_sepM_insert_2 with "").
-    { admit. }
-
-    iApply (big_sepM_insert_2 with "").
-    { admit. }
-
-    iApply (big_sepM_insert_2 with "").
-    { (* Get() handler_is *)
-      iNamed "His_shard".
-      simpl.
-      iExists _, _, _; iFrame "HgetSpec".
-
-      clear Φ.
-      iIntros (?????) "!#".
-      iIntros (Φ) "Hpre HΦ".
-      wp_pures.
-      wp_apply (wp_allocStruct).
-      { admit. } (* TODO: typecheck *)
-      iIntros (rep_ptr) "Hrep".
-      wp_pures.
-      iDestruct "Hpre" as "(Hreq_sl & Hrep_ptr & Hpre)".
-      iDestruct "Hpre" as (args) "(%Henc & #HreqInv)".
-      wp_apply (wp_decodeGetRequest with "[$Hreq_sl]").
-      { done. }
-      iIntros (args_ptr) "Hargs".
-      wp_apply (wp_GetRPC with "His_memkv [$Hargs Hrep $HreqInv]").
-      {
-        replace (zero_val (struct.t GetReply.S)) with ((#0, (slice.nil, #()))%V); last first.
-        {
-          admit. (* zero value of GetReply *)
-        }
-
-        iDestruct (struct_fields_split with "Hrep") as "HH".
-        iNamed "HH".
-        iExists (mkGetReplyC _ []).
-        iFrame.
-        iExists (Slice.nil).
-        iFrame.
-        simpl.
-        iDestruct (typed_slice.is_slice_zero byteT 1%Qp) as "HH".
-        iDestruct (typed_slice.is_slice_small_acc with "HH") as "[H _]".
-        iExists 1%Qp.
-        iFrame "H".
-      }
-      iIntros (rep') "[Hrep Hpost]".
-      wp_pures.
-      wp_apply (wp_encodeGetReply with "Hrep").
-      iIntros (repData rep_sl) "[Hrep_sl %HrepEnc]".
-      wp_store.
-      iApply "HΦ".
-      iModIntro.
-      iFrame.
-      iNext.
-      iExists _, _; iFrame.
-      done.
-    }
-
-    iApply (big_sepM_insert_2 with "").
-    { admit. }
-
-
-    iApply (big_sepM_insert_2 with "").
-    { admit. }
-
-    iApply big_sepM_empty.
-    done.
-  }
-  by iApply "HΦ".
-Admitted.
 
 End memkv_shard_proof.
 
