src/program_proof/memkv/memkv_shard_start_proof.v
@@ -1,0 +1,149 @@
+From Perennial.program_proof Require Import proof_prelude.
+From Goose.github_com.mit_pdos.gokv Require Import memkv.
+From Perennial.goose_lang Require Import ffi.grove_ffi.
+From Perennial.program_proof.lockservice Require Import rpc.
+From Perennial.program_proof.memkv Require Export memkv_shard_proof memkv_install_shard_proof common_proof.
+
+Section memkv_shard_start_proof.
+
+Context `{!heapG Σ, rpcG Σ GetReplyC}.
+
+Lemma wp_MemKVShardServer__Start (s:loc) host γ :
+is_shard_server host γ -∗
+is_MemKVShardServer s γ -∗
+  {{{
+       True
+  }}}
+    MemKVShardServer__Start #s
+  {{{
+       RET #(); True
+  }}}.
+Proof.
+  iIntros "#His_shard #His_memkv !#" (Φ) "_ HΦ".
+  wp_rec.
+  change (Alloc (InjLV (λ: <>, (λ: <>, #())%V))) with
+      (NewMap grove_common.RawRpcFunc).
+  wp_apply map.wp_NewMap.
+  iIntros (handlers_ptr) "Hmap".
+  wp_pures.
+
+  wp_apply (map.wp_MapInsert with "Hmap").
+  iIntros "Hmap".
+  wp_pures.
+
+  wp_apply (map.wp_MapInsert with "Hmap").
+  iIntros "Hmap".
+  wp_pures.
+
+  wp_apply (map.wp_MapInsert with "Hmap").
+  iIntros "Hmap".
+  wp_pures.
+
+  wp_apply (map.wp_MapInsert with "Hmap").
+  iIntros "Hmap".
+  wp_pures.
+
+  wp_apply (map.wp_MapInsert with "Hmap").
+  iIntros "Hmap".
+  wp_pures.
+
+  wp_apply (grove_ffi.wp_StartRPCServer with "[$Hmap]").
+  {
+    iApply (big_sepM_insert_2 with "").
+    { admit. }
+
+    iApply (big_sepM_insert_2 with "").
+    { (* InstallShard() handler_is *)
+      simpl.
+      iNamed "His_shard".
+      iExists _, _, _.
+      iFrame "#HinstallSpec".
+
+      clear Φ.
+      iIntros (?????) "!#".
+      iIntros (Φ) "Hpre HΦ".
+      wp_pures.
+
+      iDestruct "Hpre" as "(Hpre_sl & Hrep & Hpre)".
+      iDestruct "Hpre" as (?) "(%Hargs_enc & %HsidLe & HreqInv)".
+      wp_apply (wp_decodeInstallShardRequest with "[$Hpre_sl]").
+      { done. }
+      iIntros (args_ptr) "Hargs".
+      wp_apply (wp_InstallShardRPC with "His_memkv [$Hargs $HreqInv]").
+      {
+        done.
+      }
+      wp_pures.
+      wp_apply (typed_slice.wp_NewSlice (V:=u8)).
+      iIntros (reply_sl) "Hrep_sl".
+      wp_store.
+      iApply "HΦ".
+      iFrame.
+      done.
+    }
+
+    iApply (big_sepM_insert_2 with "").
+    { (* Get() handler_is *)
+      iNamed "His_shard".
+      simpl.
+      iExists _, _, _; iFrame "HgetSpec".
+
+      clear Φ.
+      iIntros (?????) "!#".
+      iIntros (Φ) "Hpre HΦ".
+      wp_pures.
+      wp_apply (wp_allocStruct).
+      { admit. } (* TODO: typecheck *)
+      iIntros (rep_ptr) "Hrep".
+      wp_pures.
+      iDestruct "Hpre" as "(Hreq_sl & Hrep_ptr & Hpre)".
+      iDestruct "Hpre" as (args) "(%Henc & #HreqInv)".
+      wp_apply (wp_decodeGetRequest with "[$Hreq_sl]").
+      { done. }
+      iIntros (args_ptr) "Hargs".
+      wp_apply (wp_GetRPC with "His_memkv [$Hargs Hrep $HreqInv]").
+      {
+        replace (zero_val (struct.t GetReply.S)) with ((#0, (slice.nil, #()))%V); last first.
+        {
+          admit. (* zero value of GetReply *)
+        }
+
+        iDestruct (struct_fields_split with "Hrep") as "HH".
+        iNamed "HH".
+        iExists (mkGetReplyC _ []).
+        iFrame.
+        iExists (Slice.nil).
+        iFrame.
+        simpl.
+        iDestruct (typed_slice.is_slice_zero byteT 1%Qp) as "HH".
+        iDestruct (typed_slice.is_slice_small_acc with "HH") as "[H _]".
+        iExists 1%Qp.
+        iFrame "H".
+      }
+      iIntros (rep') "[Hrep Hpost]".
+      wp_pures.
+      wp_apply (wp_encodeGetReply with "Hrep").
+      iIntros (repData rep_sl) "[Hrep_sl %HrepEnc]".
+      wp_store.
+      iApply "HΦ".
+      iModIntro.
+      iFrame.
+      iNext.
+      iExists _, _; iFrame.
+      done.
+    }
+
+    iApply (big_sepM_insert_2 with "").
+    { admit. }
+
+
+    iApply (big_sepM_insert_2 with "").
+    { admit. }
+
+    iApply big_sepM_empty.
+    done.
+  }
+  by iApply "HΦ".
+Admitted.
+
+End memkv_shard_start_proof.
